Weidenbach_Book/IsaSAT/IsaSAT_CDCL_LLVM.thy
@@ -8,13 +8,25 @@ begin
 sepref_register get_conflict_wl_is_None decide_wl_or_skip_D_heur skip_and_resolve_loop_wl_D_heur
   backtrack_wl_D_nlit_heur isasat_current_status count_decided_st_heur get_conflict_wl_is_None_heur
 
+lemma cdcl_twl_o_prog_wl_D_heurI1:
+  \<open>get_learned_count x = get_learned_count xc \<Longrightarrow>
+       learned_clss_count x < uint64_max \<Longrightarrow> learned_clss_count xc \<le> uint64_max\<close>
+  using get_learned_count_learned_clss_countD2[of xc x]
+  by (auto dest: get_learned_count_learned_clss_countD2)
+
+lemma cdcl_twl_o_prog_wl_D_heurI:
+  \<open> get_learned_count x = get_learned_count xc \<Longrightarrow>
+       learned_clss_count x < uint64_max \<Longrightarrow>  learned_clss_count xc < uint64_max\<close>
+  using get_learned_count_learned_clss_countD2[of xc x]
+  by auto
+
 sepref_def cdcl_twl_o_prog_wl_D_fast_code
   is \<open>cdcl_twl_o_prog_wl_D_heur\<close>
   :: \<open>[isasat_fast]\<^sub>a
       isasat_bounded_assn\<^sup>d \<rightarrow> bool1_assn \<times>\<^sub>a isasat_bounded_assn\<close>
   unfolding cdcl_twl_o_prog_wl_D_heur_def PR_CONST_def
   unfolding get_conflict_wl_is_None get_conflict_wl_is_None_heur_alt_def[symmetric]
-  supply [[goals_limit = 1]] isasat_fast_def[simp]
+  supply [[goals_limit = 1]] isasat_fast_def[simp] cdcl_twl_o_prog_wl_D_heurI[intro]
   apply (annot_unat_const \<open>TYPE(32)\<close>)
   by sepref
 
@@ -38,13 +50,20 @@ sepref_def length_clauses_heur_impl
 
 declare length_clauses_heur_impl.refine [sepref_fr_rules]
 
-lemma isasat_fast_alt_def: \<open>isasat_fast S = (length_clauses_heur S \<le> 9223372034707292156)\<close>
-  by (auto simp: isasat_fast_def sint64_max_def uint32_max_def length_clauses_heur_def)
+lemma isasat_fast_alt_def: \<open>isasat_fast S = (length_clauses_heur S \<le> 9223372034707292156 \<and>
+  clss_size_lcount (get_learned_count S) < 18446744073709551615 - clss_size_lcountUE (get_learned_count S) \<and>
+  clss_size_lcount (get_learned_count S) + clss_size_lcountUE (get_learned_count S) < 18446744073709551615 - clss_size_lcountUS (get_learned_count S) \<and>
+   clss_size_lcount (get_learned_count S) +
+    clss_size_lcountUE (get_learned_count S) + clss_size_lcountUS (get_learned_count S) < 18446744073709551615)\<close>
+  by (cases S; auto simp: isasat_fast_def sint64_max_def uint32_max_def length_clauses_heur_def
+    uint64_max_def learned_clss_count_def)
 
 sepref_def isasat_fast_impl
   is \<open>RETURN o isasat_fast\<close>
   :: \<open>isasat_bounded_assn\<^sup>k \<rightarrow>\<^sub>a bool1_assn\<close>
-  unfolding isasat_fast_alt_def
+  unfolding isasat_fast_alt_def short_circuit_conv
+  apply (rewrite at \<open>_ < \<hole>\<close> unat_const_fold[where 'a=64])+
+  apply (rewrite at \<open>_ < \<hole> - _\<close> unat_const_fold[where 'a=64])+
   apply (annot_snat_const \<open>TYPE(64)\<close>)
   by sepref
 
